Handle sum types

MLS.ParserTac.fst
@@ -9,11 +9,58 @@ assume new type char
 assume val ps_char: parser_serializer char
 assume val ps_unit: parser_serializer unit
 
+type nat_lbytes (sz:nat) = n:nat{n < normalize_term (pow2 (8 `op_Multiply` sz))}
+assume val ps_nat_lbytes: sz:nat -> parser_serializer (nat_lbytes sz)
+
 assume val isomorphism_explicit:
   #a:Type -> b:Type ->
   ps_a:parser_serializer a -> f:(a -> b) -> g:(b -> a) ->
   g_f_inv:(xa:a -> squash (g (f xa) == xa)) -> f_g_inv:(xb:b -> squash (f (g xb) == xb)) ->
   parser_serializer b
+
+type refined (a:Type) (pred:a -> bool) = x:a{pred x}
+
+assume val refine:
+  #a:Type ->
+  parser_serializer a -> pred:(a -> bool) -> parser_serializer (refined a pred)
+
+// `l_to_r` is so slow!
+val my_l_to_r: list term -> Tac unit
+let my_l_to_r l =
+  let squashed_equality =
+    match l with
+    | [x] -> x
+    | _ -> fail ""
+  in
+  let squashed_equality_ty = (tc (cur_env ()) squashed_equality) in
+  let x_term =
+    match inspect squashed_equality_ty with
+    | Tv_App squash_term (equality_term, Q_Explicit) -> (
+      guard (squash_term `term_eq` (`squash));
+      let eq2_term, args = collect_app equality_term in
+      guard (eq2_term `term_eq` (`eq2));
+      guard (List.Tot.length args = 3);
+      let [_; (x_term, _); _] = args in
+      guard (Tv_Var? (inspect x_term));
+      x_term
+    )
+    | _ -> fail "malformed equality"
+  in
+  let ctrl (t:term) : Tac (bool & ctrl_flag) =
+    let res =
+      match inspect t with
+      | Tv_Var _ -> t `term_eq` x_term
+      | _ -> false
+    in
+    res, Continue
+  in
+  let rw () : Tac unit =
+    apply_lemma_rw squashed_equality
+  in
+  ctrl_rewrite BottomUp ctrl rw
+
+
+(*** Utility functions ***)
 
 type parser_term = term & typ
 
@@ -47,6 +94,8 @@ val mk_const_function: typ -> term -> Tac term
 let mk_const_function ty t =
   pack (Tv_Abs (mk_binder (fresh_bv ty)) t)
 
+(*** Parser for nested pairs ***)
+
 val mk_parser_pair: parser_term -> parser_term -> Tac parser_term
 let mk_parser_pair (ps_a, t_a) (ps_b, t_b) =
   let ps_ab = mk_ie_app (quote bind) [t_a; mk_const_function t_a t_b] [ps_a; mk_const_function t_a ps_b] in
@@ -63,6 +112,8 @@ let rec mk_parser_pairs l =
     let pst_t = mk_parser_pairs t in
     mk_parser_pair pst_h pst_t
   )
+
+(*** Parser for records ***)
 
 val mkdtuple2_fv: unit -> Tac fv
 let mkdtuple2_fv () =
@@ -90,8 +141,8 @@ let mk_construct_record constructor_name bvs =
   let constructor_args = Tactics.Util.map (fun bv -> (pack (Tv_Var bv), Q_Explicit)) bvs in
   mk_app constructor_term constructor_args
 
-val mk_isomorphism_f: typ -> name -> list typ -> Tac term
-let mk_isomorphism_f result_type constructor_name constructor_types =
+val mk_record_isomorphism_f: typ -> name -> list typ -> Tac term
+let mk_record_isomorphism_f result_type constructor_name constructor_types =
   let (match_pattern, bvs) = mk_destruct_pairs constructor_types in
   let match_body = mk_construct_record constructor_name bvs in
   let x_bv = fresh_bv result_type in
@@ -105,8 +156,8 @@ let rec mk_construct_pairs l =
   | h::t ->
     mk_e_app (quote Mkdtuple2) [pack (Tv_Var h); mk_construct_pairs t]
 
-val mk_isomorphism_g: typ -> name -> list typ -> Tac term
-let mk_isomorphism_g input_type constructor_name constructor_types =
+val mk_record_isomorphism_g: typ -> name -> list typ -> Tac term
+let mk_record_isomorphism_g input_type constructor_name constructor_types =
   let bvs = Tactics.Util.map (fun t -> fresh_bv t) constructor_types in
   let match_pattern = Pat_Cons (pack_fv constructor_name) (List.Tot.map (fun bv -> (Pat_Var bv, false)) bvs) in
   let match_body = mk_construct_pairs bvs in
@@ -143,22 +194,246 @@ let prove_record_isomorphism_from_record () =
   destruct (binder_to_term b);
   let binders = intros () in
   let breq = last binders in
-  l_to_r [binder_to_term breq];
+  my_l_to_r [binder_to_term breq];
   trefl ()
 
-val mk_isomorphism: typ -> name -> list typ -> parser_term -> Tac parser_term
-let mk_isomorphism result_type constructor_name constructor_types (parser_term, parser_type) =
+val mk_record_isomorphism: typ -> name -> list typ -> parser_term -> Tac parser_term
+let mk_record_isomorphism result_type constructor_name constructor_types (parser_term, parser_type) =
   let result_parser_term =
     mk_ie_app (quote isomorphism_explicit) [parser_type] [
       result_type;
       parser_term;
-      mk_isomorphism_f parser_type constructor_name constructor_types;
-      mk_isomorphism_g result_type constructor_name constructor_types;
+      mk_record_isomorphism_f parser_type constructor_name constructor_types;
+      mk_record_isomorphism_g result_type constructor_name constructor_types;
       (`(synth_by_tactic (prove_record_isomorphism_from_pair)));
       (`(synth_by_tactic (prove_record_isomorphism_from_record)));
     ]
   in
   (result_parser_term, result_type)
+
+(*** Parser for sum type ***)
+
+// Annotation
+let with_tag (#a:Type0) (x:a) = ()
+
+val get_tag_from_annot: name -> list term -> Tac (typ & term)
+let rec get_tag_from_annot ctor_name l =
+  match l with
+  | [] -> fail ("get_tag_from_annot: no annotation for constructor " ^ (implode_qn ctor_name))
+  | h::t -> (
+    let (head, args) = collect_app h in
+    if term_eq head (`with_tag) && List.Tot.length args = 2 then (
+      let [(tag_typ, _); (tag_val, _)] = args in
+      (tag_typ, tag_val)
+    ) else (
+      get_tag_from_annot ctor_name t
+    )
+  )
+
+val get_tag_from_ctor: ctor -> Tac (typ & term)
+let get_tag_from_ctor (ctor_name, ctor_typ) =
+  match inspect ctor_typ with
+  | Tv_Arrow b _ ->
+    let _, (_, annotations) = inspect_binder b in
+    get_tag_from_annot ctor_name annotations
+  | _ -> fail "get_tag: not an arrow"
+
+val sanitize_tags: list (typ & term) -> Tac (typ & (list term))
+let sanitize_tags tags =
+  guard (Cons? tags);
+  let tag_typs, tag_vals = List.Tot.unzip tags in
+  let tag_typ =
+    guard (List.Tot.for_all (fun x -> term_eq x (Cons?.hd tag_typs)) tag_typs);
+    Cons?.hd tag_typs
+  in
+  (tag_typ, tag_vals)
+
+val mk_tag_parser: typ -> list typ -> Tac parser_term
+let mk_tag_parser tag_typ tag_vals =
+  let pred =
+    let tag_bv = fresh_bv tag_typ in
+    let tag_term = pack (Tv_Var tag_bv) in
+    let mk_disj value acc: Tac term = `(((`#tag_term) = (`#value)) || (`#acc)) in
+    guard (Cons? tag_vals);
+    let tag_vals_head::tag_vals_tail = tag_vals in
+    let disj = fold_right mk_disj tag_vals_tail (`((`#tag_term) = (`#tag_vals_head))) in
+    pack (Tv_Abs (mk_binder tag_bv) disj)
+  in
+  let (tag_parser, tag_typ) = parser_from_type tag_typ in
+  (mk_ie_app (`refine) [tag_typ] [tag_parser; pred], mk_e_app (`refined) [tag_typ; pred])
+
+
+val term_to_pattern: term -> Tac pattern
+let term_to_pattern t =
+  match inspect t with
+  | Tv_FVar fv -> Pat_Cons fv []
+  | Tv_Const c -> Pat_Constant c
+  | _ -> fail "term_to_pattern: term type not handled (not fv or const)"
+
+val mk_middle_sum_type_parser: parser_term -> list term -> list ctor -> Tac (parser_term & term)
+let mk_middle_sum_type_parser (tag_parser, tag_typ) tag_vals ctors =
+  let pair_parsers =
+    Tactics.Util.map
+      (fun (ctor_name, ctor_typ) ->
+        let types, _ = collect_arr ctor_typ in
+        mk_parser_pairs types
+      )
+      ctors
+  in
+  let (tag_to_pair_type_term, tag_to_pair_parser_term) =
+    let tag_bv = fresh_bv tag_typ in
+    let tag_term = pack (Tv_Var tag_bv) in
+    // Should be provable, but a dynamic check is enough
+    guard (List.Tot.length tag_vals = List.Tot.length pair_parsers);
+    let (branches_typ, branches_term) =
+      List.Tot.unzip (
+        Tactics.Util.map
+          (fun (tag_val, (pair_parser_term, pair_parser_typ)) -> (
+            (term_to_pattern tag_val, pair_parser_typ),
+            (term_to_pattern tag_val, pair_parser_term)
+          ))
+          (List.Pure.zip tag_vals pair_parsers)
+      )
+    in
+    (
+      pack (Tv_Abs (mk_binder tag_bv) (pack (Tv_Match tag_term None branches_typ))),
+      pack (Tv_Abs (mk_binder tag_bv) (pack (Tv_Match tag_term None branches_term)))
+    )
+  in
+  let middle_parser = mk_ie_app (`bind) [tag_typ; tag_to_pair_type_term] [tag_parser; tag_to_pair_parser_term] in
+  let middle_typ = mk_e_app (`dtuple2) [tag_typ; tag_to_pair_type_term] in
+  ((middle_parser, middle_typ), tag_to_pair_type_term)
+
+val mk_middle_to_sum_fun: typ -> term -> list term -> list ctor -> Tac term
+let mk_middle_to_sum_fun tag_typ tag_to_pair_typ tag_vals ctors =
+  guard (List.Tot.length tag_vals = List.Tot.length ctors);
+  let branches =
+    Tactics.Util.map
+      (fun (tag_val, (ctor_name, ctor_typ)) ->
+        //dump ("A " ^ term_to_string ctor_typ);
+        let types, _ = collect_arr ctor_typ in
+        let (pair_pattern, bvs) = mk_destruct_pairs types in
+        let rec_term = mk_construct_record ctor_name bvs in
+        let bvs = Tactics.Util.map (fun ty -> fresh_bv ty) types in
+        let pattern = Pat_Cons (mkdtuple2_fv ()) [(term_to_pattern tag_val, false); (pair_pattern, false)] in
+        (pattern, rec_term)
+      )
+      (List.Pure.zip tag_vals ctors)
+  in
+  //dump ("B " ^ term_to_string (mk_e_app (`dtuple2) [tag_typ; tag_to_pair_typ]));
+  let pair_bv = fresh_bv (mk_e_app (`dtuple2) [tag_typ; tag_to_pair_typ]) in
+  pack (Tv_Abs (mk_binder pair_bv) (pack (Tv_Match (pack (Tv_Var pair_bv)) None branches)))
+
+val mk_sum_to_middle_fun: typ -> list term -> list ctor -> Tac term
+let mk_sum_to_middle_fun sum_typ tag_vals ctors =
+  guard (List.Tot.length tag_vals = List.Tot.length ctors);
+  let branches =
+    Tactics.Util.map
+      (fun (tag_val, (ctor_name, ctor_typ)) ->
+        let (ctor_typs, _) = collect_arr ctor_typ in
+        let bvs = Tactics.Util.map (fun t -> fresh_bv t) ctor_typs in
+        let match_pattern = Pat_Cons (pack_fv ctor_name) (List.Tot.map (fun bv -> (Pat_Var bv, false)) bvs) in
+        let pairs_term = mk_construct_pairs bvs in
+        let match_body = mk_e_app (`Mkdtuple2) [tag_val; pairs_term] in
+        (match_pattern, match_body)
+      )
+      (List.Pure.zip tag_vals ctors)
+  in
+  //dump ("C " ^ term_to_string sum_typ);
+  let sum_bv = fresh_bv sum_typ in
+  pack (Tv_Abs (mk_binder sum_bv) (pack (Tv_Match (pack (Tv_Var sum_bv)) None branches)))
+
+val refined_ind: a:Type -> pred:(a -> bool) -> p:(a -> Type0) -> squash (forall (x:a). pred x ==> p x) -> squash (forall (x:refined a pred). p x)
+let refined_ind a pred p _ = ()
+
+val or_split: b1:bool -> b2:bool -> p:Type0 -> squash (b1 ==> p) -> squash (b2 ==> p) -> squash (b1 || b2 ==> p)
+let or_split b1 b2 p _ _ = ()
+
+val eq_to_eq: a:eqtype -> x:a -> y:a -> p:Type0 -> squash (x == y ==> p) -> squash (x = y ==> p)
+let eq_to_eq a x y p _ = ()
+let test_implies_intro_1 p q (f: squash p -> squash q)
+  : squash (p ==> q)
+  = introduce p ==> q
+    with x. f x
+
+val add_squash: p:Type0 -> q:Type0 -> squash (squash p ==> q) -> squash (p ==> q)
+let add_squash p q _ =
+  introduce p ==> q with _. ()
+
+val remove_refine: a:Type0 -> p:(a -> Type0) -> q:(a -> Type0) -> squash (forall (x:a). q x) -> squash (forall (x:a{p x}). q x)
+let remove_refine a p q _ = ()
+
+val prove_pair_sum_pair_isomorphism: unit -> Tac unit
+let prove_pair_sum_pair_isomorphism () =
+  apply (`arrow_to_forall);
+  apply_lemma (`dtuple2_ind);
+  apply (`refined_ind);
+  // TODO remove this horrible thing.
+  // Need https://github.com/FStarLang/FStar/pull/2482 to be merged first
+  compute(); let _ = repeatn 2 (fun () -> apply (`remove_refine)) in
+  let _ = forall_intro () in
+  compute ();
+  let solve_one_goal () =
+    apply (`eq_to_eq);
+    apply (`add_squash);
+    let x_eq_term = binder_to_term (implies_intro ()) in
+    my_l_to_r [x_eq_term];
+    let _ = repeat (fun () ->
+      apply_lemma (`dtuple2_ind);
+      let _ = forall_intro () in
+      ()
+    ) in
+    let _ = forall_intro () in
+    trefl()
+  in
+  let _ = repeat (fun () ->
+    apply (`or_split);
+    focus solve_one_goal
+  ) in
+  focus solve_one_goal
+
+val prove_sum_pair_sum_isomorphism: unit -> Tac unit
+let prove_sum_pair_sum_isomorphism () =
+  compute();
+  apply (`arrow_to_forall);
+  let x_term = binder_to_term (forall_intro ()) in
+  destruct x_term;
+  iterAll (fun () ->
+    let destruct_binders = intros() in
+    let breq_term = binder_to_term (last destruct_binders) in
+    my_l_to_r [breq_term];
+    compute();
+    trefl ()
+  )
+
+val mk_sum_isomorphism: typ -> typ -> term -> list term -> list ctor -> parser_term -> Tac parser_term
+let mk_sum_isomorphism tag_typ result_typ tag_to_pair_typ tag_vals ctors (pairs_parser, pairs_typ) =
+  let middle_to_sum_def = mk_middle_to_sum_fun tag_typ tag_to_pair_typ tag_vals ctors in
+  let sum_to_middle_def = mk_sum_to_middle_fun result_typ tag_vals ctors in
+  let middle_typ = mk_e_app (`dtuple2) [tag_typ; tag_to_pair_typ] in
+  let mk_a_to_b (a:typ) (b:typ) = (pack (Tv_Arrow (fresh_binder a) (pack_comp (C_Total b [])))) in
+  //We need to help F* with the type of things otherwise it is completely lost
+  let ascribe_type (t:typ) (x:term) = mk_ie_app (`id) [t] [x] in
+  let result_parser = mk_ie_app (`isomorphism_explicit) [pairs_typ] [
+    result_typ;
+    pairs_parser;
+    ascribe_type (mk_a_to_b middle_typ result_typ) middle_to_sum_def;
+    ascribe_type (mk_a_to_b result_typ middle_typ) sum_to_middle_def;
+    (`(synth_by_tactic prove_pair_sum_pair_isomorphism));
+    (`(synth_by_tactic prove_sum_pair_sum_isomorphism))
+  ] in
+  (result_parser, result_typ)
+
+val mk_sum_type_parser: list ctor -> typ -> Tac parser_term
+let mk_sum_type_parser ctors result_type =
+  let tags = Tactics.Util.map get_tag_from_ctor ctors in
+  let (tag_typ, tag_vals) = sanitize_tags tags in
+  let tag_parser_term = mk_tag_parser tag_typ tag_vals in
+  let (tag_parser, tag_typ) = tag_parser_term in
+  let (middle_sum_type_parser_term, tag_to_pair_typ) = mk_middle_sum_type_parser tag_parser_term tag_vals ctors in
+  mk_sum_isomorphism tag_typ result_type tag_to_pair_typ tag_vals ctors middle_sum_type_parser_term
+
+(*** Parser generator ***)
 
 val gen_parser_fun: term -> Tac (list binder & parser_term)
 let gen_parser_fun type_fv =
@@ -183,9 +458,12 @@ let gen_parser_fun type_fv =
       let types, _ = collect_arr c_typ in
       let pairs_parser = mk_parser_pairs types in
       let result_parsed_type = mk_e_app type_fv (Tactics.Util.map binder_to_term params) in
-      (params, mk_isomorphism result_parsed_type c_name types pairs_parser)
+      (params, mk_record_isomorphism result_parsed_type c_name types pairs_parser)
     )
-    | _ -> fail "gen_parser_fun: only records are supported"
+    | ctors -> (
+      let result_parsed_type = mk_e_app type_fv (Tactics.Util.map binder_to_term params) in
+      (params, mk_sum_type_parser ctors result_parsed_type)
+    )
   )
   | _ -> fail "gen_parser_fun: only inductives are supported"
 
@@ -199,6 +477,7 @@ let gen_parser type_fv =
   let parser_name = parser_name_from_type_name type_name in
   let (params, (parser_fun_body, parsed_type)) = gen_parser_fun type_fv in
   let parser_fun = mk_abs params parser_fun_body in
+  //dump (term_to_string parser_fun);
   let unparametrized_parser_type = mk_e_app (quote parser_serializer) [parsed_type] in
   let parser_type =
     match params with
@@ -214,6 +493,8 @@ let gen_parser type_fv =
   let sv : sigelt_view = Sg_Let false [parser_letbinding] in
   [pack_sigelt sv]
 
+(*** Tests ***)
+
 noeq type test_type2 = {
   a:char;
   b:char;
@@ -227,16 +508,23 @@ noeq type test_type2 = {
   j:char;
 }
 
-noeq type test_type3 =
-  |Test_1: char -> char -> test_type3
-  |Test_2: char -> test_type3
-
 #push-options "--fuel 0 --ifuel 0"
 %splice [ps_test_type2] (gen_parser (`test_type2))
 #pop-options
 
 assume val blbytes: nat -> Type0
 assume val ps_blbytes: n:nat -> parser_serializer (blbytes n)
+
+noeq type test_type3 =
+  | Test_1: [@@@with_tag #(nat_lbytes 1) 1] char -> char -> char -> char -> char -> char -> char -> test_type3
+  | Test_2: [@@@with_tag #(nat_lbytes 1) 2] char -> char -> char -> char -> test_type3
+  | Test_3: [@@@with_tag #(nat_lbytes 1) 3] blbytes 256 -> test_type3
+  | Test_4: [@@@with_tag #(nat_lbytes 1) 4] char -> test_type3
+  | Test_5: [@@@with_tag #(nat_lbytes 1) 5] char -> test_type3
+
+#push-options "--fuel 0 --ifuel 1"
+%splice [ps_test_type3] (gen_parser (`test_type3))
+#pop-options
 
 noeq type test_type4 = {
   a:blbytes 256;
